Start repairing thunk_to_env

compiler/backend/proofs/thunk_to_envProofScript.sml
@@ -16,140 +16,15 @@ val _ = set_grammar_ancestry ["pred_set", "rich_list", "envLang", "thunkLang",
 
 val _ = numLib.prefer_num ();
 
-(*
-Inductive exp_inv:
-  (∀v.
-     v_inv v ⇒
-       exp_inv (Value v)) ∧
-  (∀n.
-     exp_inv (Var n)) ∧
-  (∀f x.
-     exp_inv f ∧
-     exp_inv x ⇒
-       exp_inv (App f x)) ∧
-  (∀s x.
-     exp_inv x ⇒
-       exp_inv (Lam s x)) ∧
-  (∀s x y.
-     exp_inv x ∧
-     exp_inv y ⇒
-       exp_inv (Let s x y)) ∧
-  (∀x y z.
-     exp_inv x ∧
-     exp_inv y ∧
-     exp_inv z ⇒
-       exp_inv (If x y z)) ∧
-  (∀op xs.
-     EVERY exp_inv xs ⇒
-       exp_inv (Prim op xs)) ∧
-  (∀f x.
-     EVERY exp_inv (MAP SND f) ∧
-     exp_inv x ⇒
-       exp_inv (Letrec f x)) ∧
-  (∀x.
-     exp_inv x ⇒
-       exp_inv (Delay x)) ∧
-  (∀x.
-     exp_inv x ⇒
-       exp_inv (Box x)) ∧
-  (∀x.
-     exp_inv x ⇒
-       exp_inv (Force x)) ∧
-  (∀s vs.
-     EVERY v_inv vs ⇒
-       v_inv (Constructor s vs)) ∧
-  (∀s x.
-     exp_inv x ⇒
-       v_inv (Closure s x)) ∧
-  (∀f n.
-     EVERY exp_inv (MAP SND f) ⇒
-       v_inv (Recclosure f n)) ∧
-  (∀x.
-     v_inv (Atom x)) ∧
-  (∀v.
-     v_inv v ⇒
-       v_inv (Thunk (INL v))) ∧
-  (∀x.
-     exp_inv x ⇒
-       v_inv (Thunk (INR x)))
-End
-
-Theorem exp_inv_def[simp]:
-  (∀v.
-     exp_inv (Var v) = T) ∧
-  (∀v.
-     exp_inv (Value v) =
-       v_inv v) ∧
-  (∀f x.
-     exp_inv (App f x) =
-       (exp_inv f ∧ exp_inv x)) ∧
-  (∀s x.
-     exp_inv (Lam s x) =
-       exp_inv x) ∧
-  (∀s x y.
-     exp_inv (Let s x y) =
-       (exp_inv x ∧ exp_inv y)) ∧
-  (∀x y z.
-     exp_inv (If x y z) =
-       (exp_inv x ∧
-        exp_inv y ∧
-        exp_inv z)) ∧
-  (∀op xs.
-     exp_inv (Prim op xs) =
-       EVERY exp_inv xs) ∧
-  (∀f x.
-     exp_inv (Letrec f x) =
-       (EVERY exp_inv (MAP SND f) ∧
-        exp_inv x)) ∧
-  (∀x.
-     exp_inv (Delay x) =
-       exp_inv x) ∧
-  (∀x.
-     exp_inv (Box x) =
-       exp_inv x) ∧
-  (∀x.
-     exp_inv (Force x) =
-       exp_inv x) ∧
-  (∀x.
-     ¬exp_inv (MkTick x))
-Proof
-  rw [] \\ rw [Once exp_inv_cases]
-QED
-
-Theorem v_inv_def[simp]:
-  (∀s vs.
-     v_inv (Constructor s vs) =
-       EVERY v_inv vs) ∧
-  (∀s x.
-     v_inv (Closure s x) =
-       exp_inv x) ∧
-  (∀f n.
-     v_inv (Recclosure f n) =
-       EVERY exp_inv (MAP SND f)) ∧
-  (∀x.
-     v_inv (Atom x)) ∧
-  (∀v.
-     ¬v_inv (DoTick v)) ∧
-  (∀v.
-     v_inv (Thunk (INL v)) =
-       v_inv v) ∧
-  (∀x.
-     v_inv (Thunk (INR x)) =
-       exp_inv x)
-Proof
-  rw [] \\ rw [Once exp_inv_cases]
-QED
- *)
-
 Inductive exp_rel:
 [exp_rel_Value:]
   (∀env n v w.
-     ALOOKUP (REVERSE env) n = SOME w ∧
+     ALOOKUP env n = SOME w ∧
      v_rel v w ⇒
        exp_rel env (Value v) (Var n)) ∧
 [exp_rel_Var:]
   (∀env n.
-     ALOOKUP (REVERSE env) n = NONE ⇒
+     ALOOKUP env n = NONE ⇒
        exp_rel env (Var n) (Var n)) ∧
 [exp_rel_App:]
   (∀env x1 x2 y1 y2.
@@ -181,7 +56,8 @@ Inductive exp_rel:
 [exp_rel_Letrec:]
   (∀env f g x y.
      LIST_REL (λ(fn,b) (gn,c). fn = gn ∧
-                 exp_rel (FILTER (λ(n,x). ¬MEM n (MAP FST f)) env) b c) f g ∧
+                 exp_rel (FILTER (λ(n,x). ¬MEM n (MAP FST f)) env) b c)
+              f (REVERSE g) ∧
      exp_rel (FILTER (λ(n,x). ¬MEM n (MAP FST f)) env) x y ⇒
        exp_rel env (Letrec f x) (Letrec g y)) ∧
 [exp_rel_Delay:]
@@ -207,7 +83,8 @@ Inductive exp_rel:
 [v_rel_Recclosure:]
   (∀env f g n.
      LIST_REL (λ(fn,b) (gn,c). fn = gn ∧
-                 exp_rel (FILTER (λ(n,x). ¬MEM n (MAP FST f)) env) b c) f g ⇒
+                 exp_rel (FILTER (λ(n,x). ¬MEM n (MAP FST f)) env) b c)
+              f (REVERSE g) ⇒
        v_rel (Recclosure f n) (Recclosure g env n)) ∧
 [v_rel_Thunk_v:]
   (∀v w.
@@ -256,856 +133,399 @@ Theorem v_rel_def =
   |> map (SIMP_CONV (srw_ss ()) [Once v_rel_cases])
   |> LIST_CONJ;
 
-(*
-Theorem ALOOKUP_LIST_REL[local]:
-  ∀xs ys x.
-    MAP FST xs = MAP FST ys ∧
-    LIST_REL P xs ys ⇒
-      (ALOOKUP xs x = NONE ⇔ ALOOKUP ys x = NONE) ∧
-      (∀vx.
-         ALOOKUP xs x = SOME vx ⇒
-           ∃vy.
-             ALOOKUP ys x = SOME vy ∧
-             P (x, vx) (x, vy))
-Proof
-  Induct \\ simp [PULL_EXISTS, FORALL_PROD]
-  \\ rw [] \\ fs []
-QED
- *)
-
-Theorem dest_Closure_v_rel:
-  v_rel v w ⇒
-    (∀err. dest_Closure v = INL err ⇒ dest_Closure w = INL err) ∧
-    (∀s x.
-       dest_Closure v = INR (s, x) ⇒
-         ∃env y.
-           dest_Closure w = INR (s, env, y) ∧
-           exp_rel (FILTER (λ(n, x). n ≠ s) env) x y)
-Proof
-  Cases_on ‘v’ \\ Cases_on ‘w’
-  \\ simp [envLangTheory.dest_Closure_def, thunkLangTheory.dest_Closure_def,
-           v_rel_def, exp_rel_def]
-QED
-
-Theorem dest_Thunk_v_rel:
-  v_rel v w ⇒
-    (∀err. dest_Thunk v = INL err ⇒ dest_Thunk w = INL err) ∧
-    (∀nf x. dest_Thunk v = INR x ⇒
-       ∃y.
-         dest_Thunk w = INR y ∧
-           ((∃v1 v2.
-               x = INL v1 ∧
-               y = INL v2 ∧
-               v_rel v1 v2) ∨
-            (∃env x1 x2.
-               x = INR x1 ∧
-               y = INR (env, x2) ∧
-               exp_rel env x1 x2)))
-Proof
-  Cases_on ‘v’ \\ Cases_on ‘w’
-  \\ simp [envLangTheory.dest_Thunk_def, thunkLangTheory.dest_Thunk_def,
-           v_rel_def]
-  \\ Cases_on ‘s’ \\ simp [v_rel_def]
-  \\ Cases_on ‘y’ \\ simp [v_rel_def]
-QED
-
-Theorem dest_Recclosure_v_rel:
-  v_rel v w ⇒
-    (∀err. dest_Recclosure v = INL err ⇒ dest_Recclosure w = INL err) ∧
-    (∀f n.
-       dest_Recclosure v = INR (f, n) ⇒
-         ∃g env.
-           dest_Recclosure w = INR (g, env, n) ∧
-           LIST_REL (λ(fn,b) (gn,c). fn = gn ∧
-             exp_rel (FILTER (λ(n,x). ¬MEM n (MAP FST f)) env) b c) f g)
-Proof
-  Cases_on ‘v’ \\ Cases_on ‘w’
-  \\ simp [envLangTheory.dest_Recclosure_def,
-           thunkLangTheory.dest_Recclosure_def,
-           v_rel_def, exp_rel_def]
-QED
-
-Theorem dest_Constructor_v_rel:
-  v_rel v w ⇒
-    (∀err. dest_Constructor v = INL err ⇒ dest_Constructor w = INL err) ∧
-    (∀s vs.
-       dest_Constructor v = INR (s, vs) ⇒
-         ∃ws.
-           dest_Constructor w = INR (s, ws) ∧
-           LIST_REL v_rel vs ws)
-Proof
-  Cases_on ‘v’ \\ Cases_on ‘w’
-  \\ simp [envLangTheory.dest_Constructor_def,
-           thunkLangTheory.dest_Constructor_def,
-           v_rel_def, exp_rel_def]
-QED
-
 Definition env_rel_def:
-  env_rel binds env ⇔
-    MAP FST binds = MAP FST env ∧
-    ∀k v.
-      ALOOKUP (REVERSE binds) k = SOME v ⇒
-        ∃w. ALOOKUP (REVERSE env) k = SOME w ∧
-            v_rel v w
+  env_rel binds env =
+    LIST_REL (λ(f,v) (g,w). f = g ∧ v_rel v w) (REVERSE binds) env
 End
 
-Theorem exp_rel_ALOOKUP_EQ:
-  ∀env1 x y env2.
-    exp_rel env1 x y ∧
-    ALOOKUP (REVERSE env1) = ALOOKUP (REVERSE env2) ⇒
-      exp_rel env2 x y
+Theorem env_rel_OPTREL[local]:
+  env_rel binds env ⇒
+    ∀k. OPTREL v_rel (ALOOKUP (REVERSE binds) k) (ALOOKUP env k)
 Proof
-  qsuff_tac ‘
-    (∀env1 x y.
-       exp_rel env1 x y ⇒
-       ∀env2.
-         ALOOKUP (REVERSE env1) = ALOOKUP (REVERSE env2) ⇒
-         exp_rel env2 x y) ∧
-    (∀v w. v_rel v w ⇒ T)’
-  >- (
-    rw []
-    \\ first_x_assum irule
-    \\ first_assum (irule_at Any) \\ fs [])
-  \\ ho_match_mp_tac exp_rel_strongind
-  \\ simp [exp_rel_def, MEM_MAP, v_rel_def]
-  \\ rw [] \\ fs [ALOOKUP_FILTER, GSYM FILTER_REVERSE, FUN_EQ_THM]
-  \\ gvs [LIST_REL_EL_EQN]
-  \\ rw [] \\ fs []
-  \\ rpt (pairarg_tac \\ gvs [])
-  \\ first_x_assum drule \\ rw []
-  \\ first_x_assum irule \\ rw []
-  \\ fs [GSYM FILTER_REVERSE, ALOOKUP_FILTER]
-  \\ rw [] \\ gs [ALOOKUP_NONE]
+  rw [env_rel_def]
+  \\ ‘env = REVERSE (REVERSE env)’
+    by gs []
+  \\ pop_assum SUBST_ALL_TAC
+  \\ irule LIST_REL_OPTREL \\ gs []
 QED
 
-(*
-Theorem MAP_FILTER_FST[local]:
-  MAP FST (FILTER (λx. P (FST x)) xs) = FILTER (λx. P x) (MAP FST xs)
+Theorem env_rel_MAP_FST[local]:
+  env_rel binds env ⇒
+    MAP FST (REVERSE binds) = MAP FST env
 Proof
-  Induct_on ‘xs’ \\ rw []
+  rw [env_rel_def]
+  \\ irule LIST_EQ
+  \\ gvs [LIST_REL_EL_EQN, EL_MAP, EL_REVERSE, ELIM_UNCURRY]
 QED
- *)
 
 Theorem exp_rel_subst:
-  ∀env x y binds extra.
-    exp_rel env x y ∧
-    env_rel binds extra ∧
-    (∀k. MEM k (MAP FST extra) ⇒ ¬MEM k (MAP FST env)) ⇒
-      exp_rel (env ++ extra) (subst binds x) y
+  exp_rel env x y ∧
+  env_rel binds extra ∧
+  (∀k. MEM k (MAP FST extra) ⇒ ¬MEM k (MAP FST env)) ⇒
+    exp_rel (extra ++ env) (subst binds x) y
 Proof
-  qsuff_tac ‘
-    (∀env x y.
-       exp_rel env x y ⇒
-         ∀binds extra.
-           env_rel binds extra ∧
-           (∀k. MEM k (MAP FST extra) ⇒ ¬MEM k (MAP FST env)) ⇒
-             exp_rel (env ++ extra) (subst binds x) y) ∧
-    (∀v w. v_rel v w ⇒ T)’
-  >- (
-    rw [])
-  \\ ho_match_mp_tac exp_rel_strongind
-  \\ rpt conj_tac
-  \\ rpt gen_tac
-  \\ simp [subst_def, exp_rel_def]
-  >- ((* Value *)
-    rw [ALOOKUP_APPEND, REVERSE_APPEND]
-    \\ CASE_TAC \\ fs []
-    \\ dxrule_then assume_tac ALOOKUP_SOME
-    \\ dxrule_then assume_tac ALOOKUP_SOME
-    \\ gs [MAP_REVERSE])
-  >- ((* Var *)
-    rw [env_rel_def]
-    \\ CASE_TAC
-    \\ gs [exp_rel_def, ALOOKUP_APPEND, CaseEq "option", ALOOKUP_NONE,
-           MAP_REVERSE, REVERSE_APPEND]
-    \\ first_x_assum (drule_then strip_assume_tac)
-    \\ first_assum (irule_at Any) \\ fs [])
-  >- ((* Lam *)
-    rw [FILTER_APPEND_DISTRIB]
+  ‘(∀env x y.
+     exp_rel env x y ⇒
+       ∀binds extra.
+         env_rel binds extra ∧
+         (∀k. MEM k (MAP FST extra) ⇒ ¬MEM k (MAP FST env)) ⇒
+           exp_rel (extra ++ env) (subst binds x) y) ∧
+   (∀v w. v_rel v w ⇒ T)’
+   suffices_by rw []
+  \\ ho_match_mp_tac exp_rel_strongind \\ rw []
+  >~ [‘Value v’] >- (
+    dxrule_then assume_tac env_rel_OPTREL
+    \\ first_x_assum (qspec_then ‘n’ assume_tac)
+    \\ first_x_assum (qspec_then ‘n’ assume_tac)
+    \\ simp [subst_def, exp_rel_def, ALOOKUP_APPEND]
+    \\ CASE_TAC \\ gs []
+    \\ gvs [OPTREL_def, ALOOKUP_SOME, SF SFY_ss])
+  >~ [‘Var n’] >- (
+    dxrule_then assume_tac env_rel_OPTREL
+    \\ first_x_assum (qspec_then ‘n’ assume_tac)
+    \\ first_x_assum (qspec_then ‘n’ assume_tac)
+    \\ simp [subst_def]
+    \\ CASE_TAC \\ gs [exp_rel_def, OPTREL_def, ALOOKUP_NONE, ALOOKUP_APPEND])
+  >~ [‘App f x’] >- (
+    simp [subst_def, exp_rel_def])
+  >~ [‘Lam s x’] >- (
+    simp [subst_def, exp_rel_def, FILTER_APPEND_DISTRIB]
     \\ first_x_assum irule
-    \\ fs [MEM_MAP, MEM_FILTER, MAP_FILTER, EXISTS_PROD, PULL_EXISTS, SF SFY_ss]
-    \\ fs [env_rel_def, GSYM FILTER_REVERSE, ALOOKUP_FILTER, MAP_FST_FILTER])
-  >- ((* Let *)
-    rw [FILTER_APPEND_DISTRIB]
+    \\ gs [MEM_MAP, MAP_FILTER, MEM_FILTER, PULL_EXISTS, FORALL_PROD, SF SFY_ss]
+    \\ gs [env_rel_def, GSYM FILTER_REVERSE]
+    \\ qabbrev_tac ‘P = λn. n ≠ s’ \\ gs []
+    \\ irule LIST_REL_FILTER
+    \\ irule_at Any env_rel_MAP_FST \\ gs [env_rel_def, Abbr ‘P’]
+    \\ gvs [ELIM_UNCURRY, LIST_REL_EL_EQN] )
+  >~ [‘Seq x y’] >- (
+    simp [subst_def, exp_rel_def])
+  >~ [‘Let (SOME n) x y’] >- (
+    simp [subst_def, exp_rel_def, FILTER_APPEND_DISTRIB]
     \\ first_x_assum irule
-    \\ fs [MEM_MAP, MEM_FILTER, MAP_FILTER, EXISTS_PROD, PULL_EXISTS, SF SFY_ss]
-    \\ fs [env_rel_def, GSYM FILTER_REVERSE, ALOOKUP_FILTER, MAP_FST_FILTER])
-  >- ((* If *)
-    rw []
-    \\ fs [LIST_REL_EL_EQN, EL_MAP])
-  >- ((* Letrec *)
-    simp [FILTER_FILTER, MAP_MAP_o, combinTheory.o_DEF, ELIM_UNCURRY]
-    \\ strip_tac \\ rpt gen_tac \\ strip_tac
-    \\ simp [SF ETA_ss, FILTER_APPEND_DISTRIB]
-    \\ first_x_assum (irule_at Any) \\ fs []
-    \\ rpt conj_tac
-    >- (
-      fs [env_rel_def, LAMBDA_PROD, ALOOKUP_FILTER, GSYM FILTER_REVERSE,
-          MAP_FST_FILTER])
-    >- (
-      fs [LAMBDA_PROD, MAP_FST_FILTER, MEM_FILTER])
-    \\ fs [LIST_REL_EL_EQN, EL_MAP]
-    \\ rw [] \\ gvs []
-    \\ first_x_assum (drule_then strip_assume_tac) \\ fs []
-    \\ simp [FILTER_APPEND_DISTRIB] \\ gvs []
+    \\ gs [MEM_MAP, MAP_FILTER, MEM_FILTER, PULL_EXISTS, FORALL_PROD, SF SFY_ss]
+    \\ gs [env_rel_def, GSYM FILTER_REVERSE]
+    \\ qabbrev_tac ‘P = λx. x ≠ n’ \\ gs []
+    \\ irule LIST_REL_FILTER
+    \\ irule_at Any env_rel_MAP_FST \\ gs [env_rel_def, Abbr ‘P’]
+    \\ gvs [ELIM_UNCURRY, LIST_REL_EL_EQN])
+  >~ [‘If x1 y1 z1’] >- (
+    simp [subst_def, exp_rel_def])
+  >~ [‘Prim op xs’] >- (
+    simp [subst_def, exp_rel_def, EVERY2_MAP, SF ETA_ss]
+    \\ gvs [LIST_REL_EL_EQN])
+  >~ [‘Letrec f x’] >- (
+    gs [subst_def, exp_rel_def, EVERY2_MAP, FILTER_FILTER, LAMBDA_PROD,
+        MAP_MAP_o, combinTheory.o_DEF, GSYM FST_THM, FILTER_APPEND_DISTRIB]
+    \\ first_x_assum (irule_at Any)
+    \\ qabbrev_tac ‘P = λn. ¬MEM n (MAP FST f)’ \\ gs []
+    \\ gs [MAP_FST_FILTER, MEM_FILTER]
+    \\ gs [env_rel_def, GSYM FILTER_REVERSE]
+    \\ irule_at Any LIST_REL_FILTER
+    \\ irule_at Any env_rel_MAP_FST
+    \\ gs [env_rel_def]
+    \\ irule_at Any LIST_REL_mono
+    \\ first_assum (irule_at Any) \\ gs []
+    \\ irule_at Any LIST_REL_mono
+    \\ last_x_assum (irule_at Any)
+    \\ simp [FORALL_PROD] \\ rw []
     \\ first_x_assum irule
-    \\ simp [LAMBDA_PROD, MAP_FST_FILTER, MEM_FILTER]
-    \\ fs [env_rel_def, LAMBDA_PROD, ALOOKUP_FILTER, GSYM FILTER_REVERSE,
-           MAP_FST_FILTER])
+    \\ gs [MAP_FST_FILTER, GSYM FILTER_REVERSE, MEM_FILTER]
+    \\ irule LIST_REL_FILTER
+    \\ irule_at Any env_rel_MAP_FST \\ gvs [env_rel_def, LIST_REL_EL_EQN])
+  >~ [‘Delay x’] >- (
+    rw [subst_def, exp_rel_def])
+  >~ [‘Box x’] >- (
+    rw [subst_def, exp_rel_def])
+  >~ [‘Force x’] >- (
+    rw [subst_def, exp_rel_def])
 QED
 
-Theorem exp_rel_subst_app1[local]:
-  exp_rel (FILTER (λ(n,x). n ≠ s) env) b c ∧
-  v_rel v w ⇒
-    exp_rel (env ++ [(s,w)]) (subst1 s v b) c
-Proof
-  strip_tac
-  \\ irule_at Any exp_rel_ALOOKUP_EQ
-  \\ irule_at Any exp_rel_subst
-  \\ first_assum (irule_at Any) \\ simp []
-  \\ simp [env_rel_def, PULL_EXISTS, EXISTS_PROD]
-  \\ first_assum (irule_at Any)
-  \\ simp [ALOOKUP_FILTER, GSYM FILTER_REVERSE, ALOOKUP_APPEND, REVERSE_APPEND,
-           FUN_EQ_THM, MEM_MAP, MEM_FILTER, FORALL_PROD]
-QED
+Theorem SUM_REL_def[local,simp] = quotient_sumTheory.SUM_REL_def;
 
-Theorem exp_rel_subst_app2[local]:
-   exp_rel (FILTER (λ(n,x). ¬MEM n (MAP FST ys) ∧ n ≠ s) env) b c ∧
-   LIST_REL
-     (λ(fn,b) (gn,c).
-        fn = gn ∧
-        exp_rel (FILTER (λ(n,x). ¬MEM n (MAP FST ys)) env) b c) xs ys ∧
-   v_rel v w ⇒
-     exp_rel
-       (env ++ MAP (λ(f,x). (f,Recclosure ys env f)) ys ++ [(s,w)])
-       (subst (MAP (λ(g,x). (g,Recclosure xs g)) xs ++ [(s,v)]) b) c
-Proof
-  strip_tac
-  \\ ‘MAP FST xs = MAP FST ys’
-    by (qpat_x_assum ‘LIST_REL _ xs _’ mp_tac
-        \\ rpt (pop_assum kall_tac)
-        \\ rename1 ‘exp_rel foo’
-        \\ qid_spec_tac ‘ys’
-        \\ Induct_on ‘xs’ \\ Cases_on ‘ys’ \\ fs [ELIM_UNCURRY])
-  \\ irule exp_rel_ALOOKUP_EQ
-  \\ irule_at Any exp_rel_subst
-  \\ first_assum (irule_at Any) \\ simp []
-  \\ once_rewrite_tac [GSYM APPEND_ASSOC]
-  \\ qmatch_goalsub_abbrev_tac ‘REVERSE (env ++ extra1)’
-  \\ qexists_tac ‘extra1’ \\ fs [Abbr ‘extra1’]
-  \\ rpt conj_tac \\ simp []
-  >- (
-    fs [env_rel_def, MAP_MAP_o, combinTheory.o_DEF, LAMBDA_PROD, GSYM FST_THM,
-        GSYM MAP_REVERSE, ALOOKUP_APPEND, REVERSE_APPEND, ALOOKUP_MAP_2]
-    \\ rpt gen_tac
-    \\ IF_CASES_TAC \\ strip_tac \\ gvs []
-    \\ drule_then (qspec_then ‘REVERSE ys’ mp_tac) ALOOKUP_SOME_EL_2
-    \\ rw [MAP_REVERSE]
-    \\ gvs [EL_REVERSE, LIST_REL_EL_EQN, v_rel_def])
-  >- (
-    simp [MAP_MAP_o, combinTheory.o_DEF, LAMBDA_PROD, GSYM FST_THM]
-    \\ dsimp [MAP_FST_FILTER, MEM_FILTER])
-  \\ simp [FUN_EQ_THM, ALOOKUP_APPEND, REVERSE_APPEND, GSYM MAP_REVERSE,
-           GSYM FILTER_REVERSE, ALOOKUP_FILTER]
-  \\ strip_tac
-  \\ IF_CASES_TAC \\ gvs []
-  \\ CASE_TAC \\ fs []
-  \\ CASE_TAC \\ fs []
-  \\ gs [ALOOKUP_NONE, MAP_MAP_o, combinTheory.o_DEF, LAMBDA_PROD, GSYM FST_THM,
-         MAP_REVERSE]
-QED
-
-(*
-Theorem exp_inv_subst:
-  ∀ws x.
-    EVERY v_inv (MAP SND ws) ∧
-    exp_inv x ⇒
-      exp_inv (subst ws x)
-Proof
-  ho_match_mp_tac subst_ind \\ rw []
-  >- ((* Var *)
-    simp [subst_def]
-    \\ CASE_TAC \\ fs []
-    \\ dxrule_then strip_assume_tac ALOOKUP_SOME_REVERSE_EL
-    \\ gs [EVERY_EL, EL_MAP]
-    \\ first_x_assum (drule_then assume_tac) \\ gs [])
-  >- ((* Value *)
-    gvs [subst_def, EVERY_MAP, EVERY_MEM])
-  >- ((* If *)
-    gvs [subst_def])
-  >- ((* App *)
-    gvs [subst_def])
-  >- ((* Lam *)
-    gvs [subst_def]
-    \\ first_x_assum irule
-    \\ gs [EVERY_MAP, EVERY_FILTER, EVERY_MEM, ELIM_UNCURRY, SF SFY_ss])
-  >- ((* Let NONE *)
-    gvs [subst_def])
-  >- ((* Let SOME *)
-    gvs [subst_def]
-    \\ first_x_assum irule
-    \\ gs [EVERY_MAP, EVERY_FILTER, EVERY_MEM, ELIM_UNCURRY, SF SFY_ss])
-  >- ((* Letrec *)
-    gs [subst_def]
-    \\ gvs [EVERY_MAP, MAP_MAP_o, combinTheory.o_DEF, LAMBDA_PROD,
-            EVERY_FILTER, GSYM FST_THM]
-    \\ gvs [EVERY_MEM, FORALL_PROD, subst_def, SF SFY_ss])
-  >- ((* Delay *)
-    gvs [subst_def])
-  >- ((* Box *)
-    gvs [subst_def])
-  >- ((* Force *)
-    gvs [subst_def])
-  >- ((* Value *)
-    gvs [subst_def])
-QED
-       *)
+Theorem PAIR_REL_def[local,simp] = quotient_pairTheory.PAIR_REL;
 
 Theorem eval_to_exp_rel:
-  ∀k x res env y.
-    eval_to k x = res ∧
+  ∀k x env y.
     exp_rel env x y ⇒
-      case res of
-        INL err => eval_to k env y = INL err
-      | INR v => ∃w. eval_to k env y = INR w ∧ v_rel v w
+      ($= +++ v_rel) (eval_to k x) (eval_to k env y)
 Proof
-  ho_match_mp_tac eval_to_ind
-  \\ rpt conj_tac
-  \\ rpt gen_tac
-  >- ((* Value *)
-    rw [exp_rel_def]
-    \\ simp [envLangTheory.eval_to_def, thunkLangTheory.eval_to_def])
-  >- ((* Var *)
-    rw [exp_rel_def]
-    \\ simp [envLangTheory.eval_to_def, thunkLangTheory.eval_to_def ])
-  >- ((* App *)
-    rw [exp_rel_def]
-    \\ rename1 ‘exp_rel env x1 x2’
-    \\ rename1 ‘exp_rel env y1 y2’
-    \\ simp [envLangTheory.eval_to_def, thunkLangTheory.eval_to_def]
+  ho_match_mp_tac eval_to_ind \\ rw []
+  >~ [‘Value v’] >- (
+    gs [exp_rel_def, eval_to_def, envLangTheory.eval_to_def])
+  >~ [‘Var n’] >- (
+    gs [exp_rel_def, eval_to_def, envLangTheory.eval_to_def])
+  >~ [‘App f x’] >- (
+    gvs [exp_rel_def, eval_to_def, envLangTheory.eval_to_def]
+    \\ rename1 ‘exp_rel env f g’
+    \\ rename1 ‘exp_rel env x y’
     \\ first_x_assum (drule_all_then assume_tac)
     \\ first_x_assum (drule_all_then assume_tac)
-    \\ Cases_on ‘eval_to k x1’ \\ fs []
-    \\ Cases_on ‘eval_to k y1’ \\ fs []
-    \\ simp [envLangTheory.dest_anyClosure_def,
-             thunkLangTheory.dest_anyClosure_def]
-    \\ rename1 ‘eval_to k x1 = INR v1’
-    \\ qpat_x_assum ‘v_rel v1 _’ assume_tac
-    \\ drule_all_then strip_assume_tac dest_Closure_v_rel
-    \\ drule_all_then strip_assume_tac dest_Recclosure_v_rel
-    \\ Cases_on ‘dest_Recclosure v1’ \\ fs []
-    >- (
-      Cases_on ‘dest_Closure v1’ \\ gvs []
-      \\ pairarg_tac \\ gvs []
-      \\ IF_CASES_TAC \\ fs []
-      \\ first_x_assum (qspec_then ‘[]’ assume_tac) \\ fs []
-      \\ first_x_assum irule
-      \\ irule_at Any exp_rel_subst_app1 \\ fs [])
-    \\ reverse (Cases_on ‘dest_Closure v1’) \\ fs []
-    >- (
-      Cases_on ‘v1’
-      \\ fs [dest_Closure_def, dest_Recclosure_def])
-    \\ pairarg_tac \\ gvs []
-    \\ drule_then (qspec_then ‘n’ assume_tac) LIST_REL_OPTREL
-    \\ gs [OPTREL_def]
-    \\ qpat_x_assum ‘exp_rel _ x0 _’ mp_tac
-    \\ simp [Once exp_rel_cases]
-    \\ strip_tac \\ gvs []
-    \\ IF_CASES_TAC \\ fs []
-    \\ first_x_assum irule
-    \\ irule_at Any exp_rel_subst_app2 \\ fs []
-    \\ gvs [FILTER_FILTER, combinTheory.o_DEF, LAMBDA_PROD, MAP_REVERSE,
-            AC CONJ_COMM CONJ_ASSOC]
-    \\ ‘MAP FST f = MAP FST g’
-      by (irule LIST_EQ \\ gvs [LIST_REL_EL_EQN, ELIM_UNCURRY, EL_MAP])
-    \\ gs [])
-  >- ((* Lam *)
-    rw [exp_rel_def]
-    \\ simp [envLangTheory.eval_to_def, thunkLangTheory.eval_to_def,
-             v_rel_def, exp_rel_def])
-  >- ((* Let NONE *)
-    rename1 ‘Let NONE x1 y1’
-    \\ rw [exp_rel_def]
-    \\ simp [envLangTheory.eval_to_def, thunkLangTheory.eval_to_def,
-             v_rel_def, exp_rel_def]
-    \\ IF_CASES_TAC \\ fs []
-    \\ Cases_on ‘eval_to (k - 1) x1’ \\ fs []
-    \\ first_x_assum (drule_then strip_assume_tac) \\ fs []
-    \\ first_x_assum (drule_then strip_assume_tac) \\ fs [])
-  >- ((* Let SOME *)
-    rw [exp_rel_def]
-    \\ simp [envLangTheory.eval_to_def, thunkLangTheory.eval_to_def,
-             v_rel_def, exp_rel_def]
-    \\ IF_CASES_TAC \\ fs []
-    \\ Cases_on ‘eval_to (k - 1) x’ \\ fs []
-    \\ first_x_assum (drule_then strip_assume_tac) \\ fs []
-    \\ gvs []
-    \\ first_x_assum irule
-    \\ irule_at Any exp_rel_subst_app1 \\ fs [])
-  >- ((* If *)
-    rw [exp_rel_def]
-    \\ simp [envLangTheory.eval_to_def, thunkLangTheory.eval_to_def]
-    \\ IF_CASES_TAC \\ fs []
-    \\ rpt (first_x_assum (drule_then assume_tac)) \\ fs []
-    \\ Cases_on ‘eval_to (k - 1) x’ \\ fs []
-    \\ IF_CASES_TAC \\ fs []
-    >- (
-      rw []
-      \\ gvs [v_rel_def])
-    \\ IF_CASES_TAC \\ fs []
-    >- (
-      rw []
-      \\ gvs [v_rel_def])
-    \\ Cases_on ‘y’ \\ rw [] \\ gvs [v_rel_def])
-  >- ((* Letrec *)
-    rw [exp_rel_def]
-    \\ simp [envLangTheory.eval_to_def, thunkLangTheory.eval_to_def]
-    \\ IF_CASES_TAC \\ fs []
-    \\ first_x_assum irule
-    \\ fs [subst_funs_def]
-    \\ irule_at Any exp_rel_ALOOKUP_EQ
-    \\ irule_at Any exp_rel_subst
-    \\ first_assum (irule_at Any) \\ simp []
-    \\ qmatch_goalsub_abbrev_tac ‘MAP Q g’
-    \\ qexists_tac ‘MAP Q g’ \\ simp [Abbr ‘Q’]
-    \\ rename1 ‘LIST_REL _ xs ys’
-    \\ ‘MAP FST xs = MAP FST ys’
-      by (irule LIST_EQ \\ gvs [LIST_REL_EL_EQN, ELIM_UNCURRY, EL_MAP])
-    \\ rpt conj_tac
-    >- (
-      fs [env_rel_def, MAP_MAP_o, combinTheory.o_DEF, LAMBDA_PROD, GSYM FST_THM,
-          MAP_REVERSE]
-      \\ rw [GSYM MAP_REVERSE, ALOOKUP_MAP_2]
-      \\ drule_then (qspec_then ‘REVERSE ys’ mp_tac) ALOOKUP_SOME_EL_2
-      \\ simp [MAP_REVERSE]
-      \\ rw [] \\ gvs [LIST_REL_EL_EQN, EL_REVERSE, v_rel_def])
-    >- (
-      fs [MAP_MAP_o, combinTheory.o_DEF, LAMBDA_PROD, GSYM FST_THM]
-      \\ simp [MAP_FST_FILTER, MEM_FILTER])
-    \\ rw [FUN_EQ_THM, REVERSE_APPEND, GSYM FILTER_REVERSE, GSYM MAP_REVERSE,
-           ALOOKUP_APPEND, ALOOKUP_MAP_2, ALOOKUP_FILTER]
-    \\ CASE_TAC \\ fs []
-    \\ CASE_TAC \\ fs []
-    \\ gs [ALOOKUP_NONE, MAP_REVERSE])
-  >- ((* Delay *)
-    rw [exp_rel_def]
-    \\ simp [envLangTheory.eval_to_def, thunkLangTheory.eval_to_def,
-             v_rel_def])
-  >- ((* Box *)
-    rw [exp_rel_def]
-    \\ simp [envLangTheory.eval_to_def, thunkLangTheory.eval_to_def]
-    \\ Cases_on ‘eval_to k x’ \\ fs []
-    \\ first_x_assum (drule_then strip_assume_tac) \\ fs []
-    \\ simp [v_rel_def])
-  >- ((* Force *)
-    rw [exp_rel_def]
-    \\ simp [Once envLangTheory.eval_to_def, Once thunkLangTheory.eval_to_def]
+    \\ cheat (* order of evaluation *))
+  >~ [‘Lam s x’] >- (
+    gvs [exp_rel_def, eval_to_def, envLangTheory.eval_to_def, v_rel_def])
+  >~ [‘Seq x1 y1’] >- (
+    gvs [exp_rel_def, eval_to_def, envLangTheory.eval_to_def, v_rel_def]
     \\ IF_CASES_TAC \\ gs []
-    \\ Cases_on ‘eval_to k x’ \\ fs []
-    \\ first_x_assum (drule_all_then strip_assume_tac) \\ gvs []
-    \\ reverse (Cases_on ‘dest_Tick y’) \\ gs []
-    >- (
-      Cases_on ‘y’ \\ rgs [Once v_rel_cases])
-    \\ drule_all_then strip_assume_tac dest_Thunk_v_rel
-    \\ drule_all_then strip_assume_tac dest_Recclosure_v_rel
-    \\ simp [envLangTheory.dest_anyThunk_def, thunkLangTheory.dest_anyThunk_def]
-    \\ reverse (Cases_on ‘dest_Thunk y’) \\ gvs []
-    >- (
-      Cases_on ‘y’ \\ gvs []
-      \\ simp [Once envLangTheory.eval_to_def, envLangTheory.dest_anyThunk_def])
-    >- (
-      Cases_on ‘y’ \\ gvs []
-      \\ simp [Once envLangTheory.eval_to_def, envLangTheory.dest_anyThunk_def]
-      \\ first_x_assum irule
-      \\ simp [subst_funs_def])
-    \\ Cases_on ‘dest_Recclosure y’ \\ gvs []
-    \\ Cases_on ‘y’ \\ gs []
-    \\ pairarg_tac \\ gvs []
-    \\ Cases_on ‘w’ \\ gvs [v_rel_def]
-    \\ drule_then (qspec_then ‘n’ assume_tac) LIST_REL_OPTREL
-    \\ gs [OPTREL_def]
-    \\ ‘MAP FST f = MAP FST g’
-      by (irule LIST_EQ \\ gvs [LIST_REL_EL_EQN, ELIM_UNCURRY, EL_MAP])
-    \\ qpat_x_assum ‘exp_rel _ x0 _’ mp_tac
-    \\ simp [Once exp_rel_cases]
-    \\ strip_tac \\ gvs []
-    \\ simp [Once envLangTheory.eval_to_def, envLangTheory.dest_anyThunk_def]
-    \\ first_x_assum irule \\ simp []
+    \\ last_x_assum (drule_all_then assume_tac)
+    \\ Cases_on ‘eval_to (k - 1) x1’
+    \\ Cases_on ‘eval_to (k - 1) env x2’ \\ gs [])
+  >~ [‘Let (SOME n) x1 y1’] >- (
+    gvs [exp_rel_def, eval_to_def, envLangTheory.eval_to_def, v_rel_def]
+    \\ IF_CASES_TAC \\ gs []
+    \\ last_x_assum (drule_all_then assume_tac)
+    \\ Cases_on ‘eval_to (k - 1) x1’
+    \\ Cases_on ‘eval_to (k - 1) env x2’ \\ gs []
+    \\ rename1 ‘v_rel v w’
+    \\ first_x_assum irule
+    \\ ‘(n,w)::env = [n,w] ++ env’ by gs []
+    \\ pop_assum SUBST_ALL_TAC
+    \\ irule exp_rel_subst
+    (* TODO: It's OK to just filter anything we bind from env;
+             doesn't matter if its in there. The exp_rel_subst
+             theorem statement looks wrong. *)
+    \\ cheat)
+  >~ [‘If x1 y1 z1’] >- (
+    gvs [exp_rel_def, eval_to_def, envLangTheory.eval_to_def, v_rel_def]
+    \\ IF_CASES_TAC \\ gs []
+    \\ first_x_assum (drule_all_then assume_tac)
+    \\ first_x_assum (drule_all_then assume_tac)
+    \\ first_x_assum (drule_all_then assume_tac)
+    \\ Cases_on ‘eval_to (k - 1) x1’
+    \\ Cases_on ‘eval_to (k - 1) env x2’ \\ gs []
+    \\ IF_CASES_TAC \\ gs [v_rel_def]
+    \\ IF_CASES_TAC \\ gs [v_rel_def]
+    \\ IF_CASES_TAC \\ gs [v_rel_def]
+    \\ IF_CASES_TAC \\ gs [v_rel_def])
+  >~ [‘Letrec f x’] >- (
+    gvs [exp_rel_def, eval_to_def, envLangTheory.eval_to_def, v_rel_def]
+    \\ IF_CASES_TAC \\ gs []
+    \\ first_x_assum irule
     \\ simp [subst_funs_def]
-    \\ irule_at Any exp_rel_ALOOKUP_EQ
-    \\ irule_at Any exp_rel_subst
-    \\ qmatch_goalsub_abbrev_tac ‘REVERSE (env1 ++ extra1)’
-    \\ qexists_tac ‘extra1’
-    \\ first_assum (irule_at Any)
-    \\ unabbrev_all_tac
-    \\ fs [env_rel_def, MAP_MAP_o, combinTheory.o_DEF, LAMBDA_PROD, MAP_REVERSE,
-           GSYM FST_THM]
-    \\ simp [FUN_EQ_THM, GSYM MAP_REVERSE, ALOOKUP_MAP_2, GSYM FILTER_REVERSE,
-             ALOOKUP_FILTER, REVERSE_APPEND, ALOOKUP_APPEND, GSYM ALOOKUP_NONE]
-    \\ rw [] \\ rpt CASE_TAC \\ gs [ALOOKUP_NONE, PULL_EXISTS, v_rel_def,
-                                    MAP_REVERSE]
-    \\ rename1 ‘ALOOKUP (REVERSE f) k1’
-    \\ drule_then (qspec_then ‘k1’ assume_tac) LIST_REL_OPTREL
-    \\ gs [OPTREL_def])
-  >- ((* MkTick *)
-    rw [exp_rel_def]
-    \\ rgs [Once exp_rel_cases])
-  >- ((* Prim *)
-    rw [exp_rel_def]
-    \\ simp [envLangTheory.eval_to_def, thunkLangTheory.eval_to_def]
-    \\ Cases_on ‘op’ \\ fs []
+    \\ irule exp_rel_subst
+    (* TODO: Same remark as above about exp_rel_subst. *)
+    \\ cheat)
+  >~ [‘Delay x’] >- (
+    gvs [exp_rel_def, eval_to_def, envLangTheory.eval_to_def, v_rel_def])
+  >~ [‘Box x’] >- (
+    gvs [exp_rel_def, eval_to_def, envLangTheory.eval_to_def, v_rel_def]
+    \\ first_x_assum (drule_all_then assume_tac)
+    \\ rename1 ‘exp_rel _ x y’
+    \\ Cases_on ‘eval_to k x’ \\ Cases_on ‘eval_to k env y’ \\ gs [v_rel_def])
+  >~ [‘Force x’] >- (
+    gvs [exp_rel_def]
+    \\ rename1 ‘exp_rel _ x y’
+    \\ simp [Once eval_to_def, envLangTheory.eval_to_def]
+    \\ IF_CASES_TAC \\ gs []
+    \\ first_x_assum (drule_all_then assume_tac)
+    \\ gs [PULL_EXISTS]
+    \\ Cases_on ‘eval_to k x’ \\ Cases_on ‘eval_to k env y’ \\ gs []
+    \\ rename1 ‘v_rel v w’
+    \\ reverse (Cases_on ‘dest_Tick v’) \\ gs []
+    >- (
+      Cases_on ‘v’ \\ gs []
+      \\ rgs [Once v_rel_cases])
+    \\ Cases_on ‘v’ \\ Cases_on ‘w’ \\ gvs [dest_anyThunk_def, v_rel_def,
+                                           envLangTheory.dest_anyThunk_def]
+    >- (
+      qmatch_asmsub_abbrev_tac
+        ‘LIST_REL (λ(a,x) (b,y). a = b ∧ R x y) xs (REVERSE ys)’
+      \\ ‘OPTREL R (ALOOKUP (REVERSE xs) s) (ALOOKUP ys s)’
+        by (‘ys = REVERSE (REVERSE ys)’
+              by gs []
+            \\ pop_assum SUBST1_TAC
+            \\ irule LIST_REL_OPTREL \\ gs [])
+      \\ gvs [OPTREL_def, Abbr ‘R’]
+      \\ pop_assum mp_tac
+      \\ rw [Once exp_rel_cases] \\ gs []
+      \\ first_x_assum irule
+      \\ gs [subst_funs_def]
+      \\ irule exp_rel_subst
+      \\ cheat (* exp_rel_subst *))
+    \\ CASE_TAC \\ gvs [v_rel_def]
+    \\ first_x_assum irule
+    \\ simp [subst_funs_def])
+  >~ [‘MkTick x’] >- (
+    rgs [Once exp_rel_cases])
+  >~ [‘Prim op xs’] >- (
+    gvs [exp_rel_def, eval_to_def, envLangTheory.eval_to_def]
+    \\ Cases_on ‘op’ \\ gs []
     >- ((* Cons *)
-      gvs [LIST_REL_EL_EQN, MEM_EL, PULL_EXISTS]
+      gvs [LIST_REL_EL_EQN, MEM_EL, PULL_EXISTS, SF ETA_ss]
       \\ qmatch_goalsub_abbrev_tac ‘result_map f xs’
       \\ qmatch_goalsub_abbrev_tac ‘result_map g ys’
-      \\ Cases_on ‘result_map f xs’ \\ fs []
+      \\ ‘($= +++ (LIST_REL v_rel)) (result_map f xs) (result_map g ys)’
+        suffices_by (
+          rw []
+          \\ Cases_on ‘result_map f xs’ \\ Cases_on ‘result_map g ys’ \\ gs []
+          \\ simp [v_rel_def])
+      \\ gs [result_map_def, MEM_EL, PULL_EXISTS, EL_MAP, SF CONJ_ss]
+      \\ unabbrev_all_tac
+      \\ IF_CASES_TAC \\ gs []
       >- (
-        reverse (Cases_on ‘result_map g ys’) \\ fs []
-        >- (
-          gvs [result_map_def, CaseEq "bool", MEM_MAP]
-          \\ fs [Once (DECIDE “A ⇒ ¬B ⇔ B ⇒ ¬A”)]
-          \\ unabbrev_all_tac
-          \\ gs [MEM_EL, PULL_EXISTS]
-          \\ rpt (first_x_assum (drule_then assume_tac)) \\ gs [EVERY_EL])
-        \\ rgs [result_map_def, CaseEq "bool", MEM_MAP] \\ gvs []
-        \\ fs [Once (DECIDE “A ⇒ ¬B ⇔ B ⇒ ¬A”)]
-        \\ unabbrev_all_tac \\ rgs []
-        \\ rgs [MEM_EL, PULL_EXISTS] \\ gvs []
-        >- (
-          rpt (first_x_assum (drule_then assume_tac)) \\ gs [EVERY_EL]
-          \\ pop_assum mp_tac \\ gs []
-          \\ CASE_TAC \\ rgs [])
-        \\ rename1 ‘eval_to k (EL m xs)’
-        \\ qpat_x_assum ‘m < LENGTH ys’ assume_tac
-        \\ rpt (first_x_assum (drule_then assume_tac)) \\ gs [EVERY_EL])
-      \\ Cases_on ‘result_map g ys’ \\ gs []
+        first_x_assum (drule_then assume_tac)
+        \\ first_x_assum (drule_all_then assume_tac)
+        \\ Cases_on ‘eval_to k env (EL n ys)’ \\ gvs [SF SFY_ss])
+      \\ gs [DECIDE “A ⇒ ¬(B < C) ⇔ B < C ⇒ ¬A”]
+      \\ IF_CASES_TAC \\ gs []
       >- (
-        gvs [result_map_def, CaseEq "bool", MEM_MAP, MEM_EL, PULL_EXISTS,
-             EVERY_EL]
-        \\ fs [Once (DECIDE “A ⇒ ¬B ⇔ B ⇒ ¬A”)]
-        \\ unabbrev_all_tac \\ gs []
-        \\ rpt (first_x_assum (drule_all_then assume_tac))
-        \\ pop_assum mp_tac
-        \\ CASE_TAC \\ gs []
-        \\ strip_tac \\ gs [])
-      \\ gvs [v_rel_def, LIST_REL_EL_EQN, result_map_def, CaseEq "bool",
-              MEM_MAP, EVERY_EL, EL_MAP]
-      \\ fs [Once (DECIDE “A ⇒ ¬B ⇔ B ⇒ ¬A”)]
-      \\ gs [MAP_MAP_o, combinTheory.o_DEF, EL_MAP] \\ rw []
-      \\ gvs [MEM_EL, PULL_EXISTS]
-      \\ rpt (first_x_assum (drule_all_then assume_tac))
+        last_assum (drule_all_then assume_tac)
+        \\ last_assum (drule_all_then assume_tac)
+        \\ Cases_on ‘eval_to k env (EL n ys)’ \\ gvs [SF SFY_ss]
+        \\ IF_CASES_TAC \\ gs []
+        \\ rename1 ‘m < LENGTH ys’
+        \\ first_x_assum (drule_all_then assume_tac)
+        \\ first_x_assum (drule_all_then assume_tac)
+        \\ Cases_on ‘eval_to k (EL m xs)’ \\ gs [])
+      \\ gs [DECIDE “A ⇒ ¬(B < C) ⇔ B < C ⇒ ¬A”]
+      \\ IF_CASES_TAC \\ gs []
+      >- (
+        first_x_assum (drule_all_then assume_tac)
+        \\ first_x_assum (drule_all_then assume_tac)
+        \\ first_x_assum (drule_then assume_tac)
+        \\ first_x_assum (drule_then assume_tac)
+        \\ Cases_on ‘eval_to k (EL n xs)’ \\ gs [])
+      \\ gs [DECIDE “A ⇒ ¬(B < C) ⇔ B < C ⇒ ¬A”]
+      \\ IF_CASES_TAC \\ gs []
+      >- (
+        first_x_assum (drule_all_then assume_tac)
+        \\ first_x_assum (drule_all_then assume_tac)
+        \\ first_x_assum (drule_then assume_tac)
+        \\ first_x_assum (drule_then assume_tac)
+        \\ Cases_on ‘eval_to k (EL n xs)’ \\ gs [])
+      \\ gvs [DECIDE “A ⇒ ¬(B < C) ⇔ B < C ⇒ ¬A”, EVERY2_MAP, LIST_REL_EL_EQN]
+      \\ rw []
+      \\ first_x_assum (drule_all_then assume_tac)
+      \\ first_x_assum (drule_all_then assume_tac)
       \\ rpt (first_x_assum (drule_then assume_tac))
-      \\ unabbrev_all_tac \\ gs []
-      \\ Cases_on ‘eval_to k (EL n xs)’ \\ Cases_on ‘eval_to k env (EL n ys)’
-      \\ gvs []
-      \\ rename1 ‘INL err’
-      \\ Cases_on ‘err’ \\ gs [])
+      \\ Cases_on ‘eval_to k (EL n xs)’
+      \\ Cases_on ‘eval_to k env (EL n ys)’ \\ gs []
+      \\ rename1 ‘INL err’ \\ Cases_on ‘err’ \\ gs [])
     >- ((* IsEq *)
       gvs [LIST_REL_EL_EQN]
-      \\ IF_CASES_TAC \\ fs []
+      \\ IF_CASES_TAC \\ gs []
       \\ gvs [LENGTH_EQ_NUM_compute, DECIDE “∀n. n < 1 ⇔ n = 0”]
-      \\ IF_CASES_TAC \\ fs []
-      \\ rename1 ‘eval_to (k - 1) x’
-      \\ Cases_on ‘eval_to (k - 1) x’ \\ fs []
+      \\ IF_CASES_TAC \\ gs []
+      \\ rename1 ‘exp_rel env x y’
       \\ first_x_assum (drule_then strip_assume_tac)
-      \\ drule_all_then strip_assume_tac dest_Constructor_v_rel
-      \\ Cases_on ‘dest_Constructor y’ \\ fs []
-      \\ pairarg_tac \\ gvs []
-      \\ imp_res_tac LIST_REL_LENGTH
-      \\ IF_CASES_TAC \\ fs []
-      \\ simp [v_rel_def])
+      \\ Cases_on ‘eval_to (k - 1) x’
+      \\ Cases_on ‘eval_to (k - 1) env y’ \\ gs []
+      \\ rename1 ‘v_rel v w’
+      \\ Cases_on ‘v’ \\ Cases_on ‘w’ \\ gvs [v_rel_def]
+      \\ gvs [LIST_REL_EL_EQN]
+      \\ IF_CASES_TAC \\ gs [v_rel_def])
     >- ((* Proj *)
       gvs [LIST_REL_EL_EQN]
-      \\ IF_CASES_TAC \\ fs []
+      \\ IF_CASES_TAC \\ gs []
       \\ gvs [LENGTH_EQ_NUM_compute, DECIDE “∀n. n < 1 ⇔ n = 0”]
-      \\ IF_CASES_TAC \\ fs []
-      \\ rename1 ‘eval_to (k - 1) x’
-      \\ Cases_on ‘eval_to (k - 1) x’ \\ fs []
+      \\ IF_CASES_TAC \\ gs []
+      \\ rename1 ‘exp_rel env x y’
       \\ first_x_assum (drule_then strip_assume_tac)
-      \\ drule_all_then strip_assume_tac dest_Constructor_v_rel
-      \\ Cases_on ‘dest_Constructor y’ \\ fs []
-      \\ pairarg_tac \\ gvs [LIST_REL_EL_EQN]
-      \\ IF_CASES_TAC \\ fs []
-      \\ Cases_on ‘y’ \\ gvs [EVERY_EL])
+      \\ Cases_on ‘eval_to (k - 1) x’
+      \\ Cases_on ‘eval_to (k - 1) env y’ \\ gs []
+      \\ rename1 ‘v_rel v w’
+      \\ Cases_on ‘v’ \\ Cases_on ‘w’ \\ gvs [v_rel_def]
+      \\ gvs [LIST_REL_EL_EQN]
+      \\ IF_CASES_TAC \\ gs [v_rel_def])
     >- ((* AtomOp *)
       gvs [LIST_REL_EL_EQN, MEM_EL, PULL_EXISTS]
       \\ Cases_on ‘k = 0’ \\ gs []
       >- (
         simp [result_map_def, MEM_MAP, GSYM NOT_NULL_MEM, NULL_EQ]
-        \\ IF_CASES_TAC \\ gs []
-        >- (
-          IF_CASES_TAC \\ gs [])
+        \\ rw [] \\ gvs []
         \\ CASE_TAC \\ gs []
         \\ CASE_TAC \\ gs [v_rel_def])
       \\ qmatch_goalsub_abbrev_tac ‘result_map f xs’
       \\ qmatch_goalsub_abbrev_tac ‘result_map g ys’
-      \\ qsuff_tac ‘result_map f xs = result_map g ys’
-      >- (
-        rw []
-        \\ Cases_on ‘result_map g ys’ \\ gs []
-        \\ CASE_TAC \\ gs []
-        \\ CASE_TAC \\ gs [v_rel_def])
-      \\ rgs [result_map_def, MEM_MAP, EVERY_EL]
+      \\ ‘result_map f xs = result_map g ys’
+        suffices_by (
+          rw []
+          \\ Cases_on ‘result_map g ys’ \\ gs []
+          \\ CASE_TAC \\ gs []
+          \\ CASE_TAC \\ gs [v_rel_def])
+      \\ gs [result_map_def, MEM_EL, PULL_EXISTS, EL_MAP, SF CONJ_ss]
+      \\ unabbrev_all_tac
       \\ IF_CASES_TAC \\ gs []
       >- (
-        IF_CASES_TAC \\ gs []
-        \\ fs [Once (DECIDE “A ⇒ ¬B ⇔ B ⇒ ¬A”)]
-        \\ gvs [MEM_EL, PULL_EXISTS]
-        \\ first_x_assum (drule_then assume_tac)
-        \\ unabbrev_all_tac \\ gs []
-        \\ rpt (first_x_assum (drule_then assume_tac))
-        \\ gvs [CaseEqs ["sum", "v"]]
-        \\ rename1 ‘v_rel _ w’ \\ Cases_on ‘w’ \\ gs [v_rel_def])
+        first_x_assum (drule_then assume_tac)
+        \\ first_x_assum (drule_all_then assume_tac)
+        \\ rw [] \\ gs [DECIDE “A ⇒ ¬(B < C) ⇔ B < C ⇒ ¬A”]
+        \\ rpt (first_x_assum (qspec_then ‘n’ assume_tac)) \\ gs []
+        \\ Cases_on ‘eval_to (k - 1) (EL n xs)’
+        \\ Cases_on ‘eval_to (k - 1) env (EL n ys)’ \\ gs []
+        \\ rename1 ‘v_rel v w’
+        \\ Cases_on ‘v’ \\ Cases_on ‘w’ \\ gs [v_rel_def])
+      \\ gs [DECIDE “A ⇒ ¬(B < C) ⇔ B < C ⇒ ¬A”]
       \\ IF_CASES_TAC \\ gs []
       >- (
-        reverse IF_CASES_TAC \\ gs []
+        rw [] \\ gs [DECIDE “A ⇒ ¬(B < C) ⇔ B < C ⇒ ¬A”]
         >- (
-          fs [Once (DECIDE “A ⇒ ¬B ⇔ B ⇒ ¬A”)]
-          \\ gvs [MEM_EL, PULL_EXISTS]
-          \\ first_x_assum (drule_then assume_tac)
-          \\ unabbrev_all_tac \\ gs []
-          \\ rpt (first_x_assum (drule_then assume_tac))
-          \\ first_assum (irule_at Any) \\ gs []
-          \\ pop_assum mp_tac
-          \\ rpt CASE_TAC \\ gs [CaseEqs ["v"], v_rel_def])
-        \\ unabbrev_all_tac \\ gs []
-        \\ rgs [MEM_EL, PULL_EXISTS] \\ gvs []
-        \\ rpt (first_x_assum (drule_then assume_tac))
-        \\ pop_assum mp_tac
-        \\ rpt CASE_TAC \\ gs []
-        >- (
-          strip_tac \\ gs [CaseEqs ["sum", "envLang$v"]])
-        \\ rw [DISJ_EQ_IMP]
-        \\ strip_tac
-        \\ last_x_assum (qspec_then ‘EL n xs’ assume_tac)
-        \\ gs [CaseEqs ["sum", "envLang$v", "v"]]
-        \\ Cases_on ‘y’ \\ gvs [v_rel_def])
-      \\ IF_CASES_TAC \\ gs []
+          rename1 ‘m < LENGTH ys’
+          \\ last_x_assum (drule_all_then assume_tac)
+          \\ last_x_assum (drule_all_then assume_tac)
+          \\ rpt (first_x_assum (qspec_then ‘m’ assume_tac)) \\ gs []
+          \\ Cases_on ‘eval_to (k - 1) (EL m xs)’
+          \\ Cases_on ‘eval_to (k - 1) env (EL m ys)’ \\ gs []
+          \\ rename1 ‘v_rel v w’
+          \\ Cases_on ‘v’ \\ Cases_on ‘w’ \\ gs [v_rel_def])
+        \\ last_x_assum (drule_all_then assume_tac)
+        \\ last_x_assum (drule_all_then assume_tac)
+        \\ rpt (first_x_assum (qspec_then ‘n’ assume_tac)) \\ gs []
+        \\ Cases_on ‘eval_to (k - 1) (EL n xs)’
+        \\ Cases_on ‘eval_to (k - 1) env (EL n ys)’ \\ gs []
+        \\ rename1 ‘v_rel v w’
+        \\ Cases_on ‘v’ \\ Cases_on ‘w’ \\ gs [v_rel_def])
+      \\ rw [] \\ gs [DECIDE “A ⇒ ¬(B < C) ⇔ B < C ⇒ ¬A”]
       >- (
-        fs [Once (DECIDE “A ⇒ ¬B ⇔ B ⇒ ¬A”)]
-        \\ unabbrev_all_tac
-        \\ rgs [MEM_EL, PULL_EXISTS] \\ gvs []
+        first_x_assum (drule_all_then assume_tac)
+        \\ first_x_assum (drule_all_then assume_tac)
         \\ rpt (first_x_assum (drule_then assume_tac))
-        \\ pop_assum mp_tac
-        \\ rpt CASE_TAC \\ gs []
-        >- (
-          strip_tac \\ gs [CaseEqs ["sum", "envLang$v"]])
-        \\ rw [DISJ_EQ_IMP]
-        \\ strip_tac
-        \\ gs [CaseEqs ["sum", "envLang$v", "v"]]
-        \\ Cases_on ‘y’ \\ gvs [v_rel_def])
-      \\ fs [Once (DECIDE “A ⇒ ¬B ⇔ B ⇒ ¬A”)]
-      \\ gs [EL_MAP, MEM_EL, PULL_EXISTS]
-      \\ unabbrev_all_tac \\ gs [] \\ rw []
+        \\ Cases_on ‘eval_to (k - 1) (EL n xs)’
+        \\ Cases_on ‘eval_to (k - 1) env (EL n ys)’ \\ gs []
+        \\ rename1 ‘v_rel v w’
+        \\ Cases_on ‘v’ \\ Cases_on ‘w’ \\ gs [v_rel_def])
       >- (
-        rpt (first_x_assum (drule_then assume_tac))
-        \\ pop_assum mp_tac
-        \\ CASE_TAC \\ gs [] \\ rw []
-        \\ gs [CaseEqs ["envLang$v", "v"]]
-        \\ rename1 ‘v_rel v1 v2’
-        \\ Cases_on ‘v1’ \\ Cases_on ‘v2’ \\ gs [v_rel_def])
-      \\ simp [MAP_MAP_o, combinTheory.o_DEF]
+        first_x_assum (drule_all_then assume_tac)
+        \\ first_x_assum (drule_all_then assume_tac)
+        \\ rpt (first_x_assum (drule_then assume_tac))
+        \\ Cases_on ‘eval_to (k - 1) (EL n xs)’
+        \\ Cases_on ‘eval_to (k - 1) env (EL n ys)’ \\ gs []
+        \\ rename1 ‘v_rel v w’
+        \\ Cases_on ‘v’ \\ Cases_on ‘w’ \\ gs [v_rel_def])
       \\ irule LIST_EQ
-      \\ gvs [EL_MAP] \\ rw []
+      \\ gs [MAP_MAP_o, combinTheory.o_DEF, EL_MAP]
+      \\ qx_gen_tac ‘m’ \\ rw []
+      \\ first_x_assum (drule_all_then assume_tac)
+      \\ first_x_assum (drule_all_then assume_tac)
       \\ rpt (first_x_assum (drule_then assume_tac))
-      \\ CASE_TAC \\ gs []
-      \\ CASE_TAC \\ gs []
-      \\ CASE_TAC \\ gs [v_rel_def]))
+      \\ Cases_on ‘eval_to (k - 1) (EL m xs)’
+      \\ Cases_on ‘eval_to (k - 1) env (EL m ys)’ \\ gs []
+      \\ rename1 ‘v_rel v w’
+      \\ Cases_on ‘v’ \\ Cases_on ‘w’ \\ gs [v_rel_def]))
 QED
 
 Theorem eval_exp_rel:
-  eval x = res ∧
   exp_rel env x y ⇒
-    case res of
-      INL err => eval env y = INL err
-    | INR v => ∃w. eval env y = INR w ∧ v_rel v w
+    ($= +++ v_rel) (eval x) (eval env y)
 Proof
   rw [thunkLangTheory.eval_def, envLangTheory.eval_def]
+  \\ DEEP_INTRO_TAC some_intro
   \\ DEEP_INTRO_TAC some_intro \\ simp []
-  \\ reverse strip_tac
-  >- (
-    strip_tac
-    \\ DEEP_INTRO_TAC some_intro \\ simp []
-    \\ qx_gen_tac ‘k’
-    \\ ‘∃r. eval_to k x = r’ by fs []
-    \\ drule_all eval_to_exp_rel \\ gs [])
-  \\ qx_gen_tac ‘k’
-  \\ strip_tac
-  \\ DEEP_INTRO_TAC some_intro \\ simp []
-  \\ reverse strip_tac
-  >- (
-    strip_tac
-    \\ ‘∃r. eval_to k x = r’ by fs []
-    \\ drule_all eval_to_exp_rel \\ gs [])
+  \\ simp [PULL_FORALL]
+  \\ qx_gen_tac ‘i’
   \\ qx_gen_tac ‘j’
-  \\ strip_tac
-  \\ ‘∃r. eval_to k x = r’ by fs []
-  \\ drule_all_then assume_tac eval_to_exp_rel
-  \\ Cases_on ‘j ≤ k’ \\ gvs []
+  \\ qx_gen_tac ‘k’
+  \\ rw [] \\ gs []
   >- (
-    drule_all envLangTheory.eval_to_mono
-    \\ disch_then (assume_tac o SYM)
+    drule_all_then (qspec_then ‘i + j’ assume_tac) eval_to_exp_rel
+    \\ drule_then (qspec_then ‘i + j’ assume_tac) eval_to_mono
+    \\ drule_then (qspec_then ‘i + j’ assume_tac) envLangTheory.eval_to_mono
     \\ gs [])
-  \\ ‘k ≤ j’ by fs []
-  \\ drule_all thunkLangTheory.eval_to_mono
-  \\ disch_then (assume_tac o SYM) \\ gs []
-  \\ irule_at Any eval_to_exp_rel
-  \\ irule_at Any EQ_REFL \\ fs []
-QED
-
-(*
-Theorem compile_exp_freevars:
-  ∀x. freevars (compile_exp x) = freevars x
-Proof
-  ho_match_mp_tac compile_exp_ind
-  \\ rpt conj_tac
-  \\ rpt gen_tac
-  \\ simp [compile_exp_def, envLangTheory.freevars_def,
-           thunkLangTheory.freevars_def]
-  \\ rpt strip_tac
   >- (
-    simp [MAP_MAP_o, combinTheory.o_DEF]
-    \\ AP_TERM_TAC
-    \\ AP_TERM_TAC
-    \\ irule LIST_EQ
-    \\ gvs [MEM_EL, PULL_EXISTS, EL_MAP, EVERY_EL])
-  >- (
-    rename1 ‘Let opt _ _’
-    \\ Cases_on ‘opt’ \\ gs [envLangTheory.freevars_def,
-                             thunkLangTheory.freevars_def])
-  >- (
-    rw [MEM_MAP, MAP_MAP_o, combinTheory.o_DEF, EXTENSION, EVERY_MEM]
-    \\ fs [EXISTS_PROD, FORALL_PROD]
-    \\ metis_tac [])
+    drule_all_then (qspec_then ‘i’ assume_tac) eval_to_exp_rel
+    \\ first_x_assum (qspec_then ‘i’ assume_tac) \\ gs [])
+  \\ drule_all_then (qspec_then ‘k’ assume_tac) eval_to_exp_rel
+  \\ first_x_assum (qspec_then ‘k’ assume_tac) \\ gs []
 QED
- *)
-
-(*
-Theorem compile_exp_closed:
-  ∀x. closed (compile_exp x) = closed x
-Proof
-  rw [envLangTheory.closed_def, thunkLangTheory.closed_def,
-      compile_exp_freevars]
-QED
- *)
-
-(*
- * No values, but also no MkTicks.
- *)
-(*
-Definition no_Value_def:
-  no_Value (Value v) = F ∧
-  no_Value (Var n) = T ∧
-  no_Value (Prim op xs) = EVERY no_Value xs ∧
-  no_Value (App x y) = (no_Value x ∧ no_Value y) ∧
-  no_Value (Lam s x) = no_Value x ∧
-  no_Value (Let s x y) = (no_Value x ∧ no_Value y) ∧
-  no_Value (Letrec f x) =
-    (EVERY (λ(f,x). no_Value x) f ∧
-     no_Value x) ∧
-  no_Value (If x y z) = (no_Value x ∧ no_Value y ∧ no_Value z) ∧
-  no_Value (Delay x) = no_Value x ∧
-  no_Value (Box x) = no_Value x ∧
-  no_Value (Force x) = no_Value x ∧
-  no_Value (MkTick x) = F (* no_Value x *)
-Termination
-  WF_REL_TAC ‘measure exp_size’ \\ simp []
-  \\ rw [] \\ rename1 ‘MEM _ xs’
-  \\ Induct_on ‘xs’ \\ rw [] \\ fs [thunkLangTheory.exp_size_def]
-End
-*)
-
-(*
-Theorem exp_inv_rce:
-  ∀x. exp_inv (rce x)
-Proof
-  ho_match_mp_tac rce_ind
-  \\ rw [rce_def]
-  \\ gs [EVERY_MEM, MEM_MAP, FORALL_PROD, EXISTS_PROD, PULL_EXISTS, SF SFY_ss]
-QED
-
-Theorem no_Value_exp_inv:
-  ∀x. no_Value x ⇒ exp_inv x
-Proof
-  ho_match_mp_tac exp_ind
-  \\ rw [] \\ gs [no_Value_def]
-  \\ gs [EVERY_MEM, MEM_MAP, EXISTS_PROD, PULL_EXISTS, FORALL_PROD, SF SFY_ss]
-QED
-
-Theorem compile_exp_rce:
-  ∀x. no_Value x ⇒ rce (compile_exp x) = x
-Proof
-  ho_match_mp_tac compile_exp_ind
-  \\ simp [rce_def, no_Value_def, compile_exp_def] \\ rw []
-  \\ fs [MAP_MAP_o, combinTheory.o_DEF, EVERY_MEM]
-  \\ irule MAP_ID_ON \\ fs []
-  \\ fs [ELIM_UNCURRY, FORALL_PROD, SF SFY_ss]
-QED
-
-Theorem exp_rel_rce:
-  ∀x. exp_rel [] (rce x) x
-Proof
-  ho_match_mp_tac rce_ind
-  \\ simp [rce_def, exp_rel_def]
-  \\ rw []
-  \\ fs [EVERY2_MAP, LIST_REL_EL_EQN, MEM_EL, PULL_EXISTS, EL_MAP] \\ rw []
-  >- (
-    rename1 ‘Let opt _ _’
-    \\ Cases_on ‘opt’ \\ fs [exp_rel_def])
-  \\ fs [ELIM_UNCURRY]
-  \\ first_x_assum irule
-  \\ first_assum (irule_at Any) \\ fs []
-  \\ irule_at Any PAIR
-QED
-
-Theorem eval_to_rce:
-  eval_to k (rce x) = res ⇒
-  case res of
-    INL err => eval_to k [] x = INL err
-  | INR v => ∃w. eval_to k [] x = INR w ∧ v_rel v w ∧ v_inv v
-Proof
-  strip_tac
-  \\ irule_at Any eval_to_exp_rel
-  \\ irule_at Any exp_rel_rce \\ fs []
-  \\ irule exp_inv_rce
-QED
-
-Theorem eval_rce:
-  eval (rce x) = res ⇒
-  case res of
-    INL err => eval [] x = INL err
-  | INR v => ∃w. eval [] x = INR w ∧ v_rel v w ∧ v_inv v
-Proof
-  strip_tac
-  \\ irule_at Any eval_exp_rel
-  \\ irule_at Any exp_rel_rce \\ fs []
-  \\ irule exp_inv_rce
-QED
-
-Theorem compile_exp_eval_to:
-  eval_to k x = res ∧
-  no_Value x ⇒
-    case res of
-      INL err => eval_to k [] (compile_exp x) = INL err
-    | INR v => ∃w. eval_to k [] (compile_exp x) = INR w ∧ v_rel v w ∧ v_inv v
-Proof
-  strip_tac
-  \\ irule eval_to_rce
-  \\ simp [compile_exp_rce]
-QED
-
-Theorem compile_exp_eval:
-  eval x = res ∧
-  no_Value x ⇒
-    case res of
-      INL err => eval [] (compile_exp x) = INL err
-    | INR v => ∃w. eval [] (compile_exp x) = INR w ∧ v_rel v w ∧ v_inv v
-Proof
-  strip_tac
-  \\ irule eval_rce
-  \\ simp [compile_exp_rce]
-QED
- *)
 
 val _ = export_theory ();
 
